finalization and cleanup

Syntax.v
@@ -1,5 +1,5 @@
-Require Import Coq.Strings.String.
 Require Import Maps.
+Require Import Coq.Strings.String.
 Require Coq.Lists.ListSet.
 
 
@@ -46,46 +46,20 @@ Definition idEmpty {V: Type} := p_empty id V.
 Definition idUpdate {V: Type} (k: id) (v: V) (m: idMap V): idMap V :=
   p_update (fun x y => if id_dec x y then true else false) m k v.
 
-Example test_idEmpty_1: (@idEmpty nat) (Id "x") = None.
-Proof. reflexivity. Qed.
-
-Example test_update_1: (idUpdate (Id "x") 1 idEmpty) (Id "x") = Some 1. 
-Proof. reflexivity. Qed.
-Example test_update_2: (idUpdate (Id "x") 1 idEmpty) (Id "y") = None.  
-Proof. reflexivity. Qed.
-Example test_update_3: (idUpdate (Id "x") 2 (idUpdate (Id "x") 1 idEmpty) (Id "x")) = Some 2.
-Proof. reflexivity. Qed.
-Example test_update_4: (idUpdate (Id "y") 2 (idUpdate (Id "x") 1 idEmpty) (Id "x")) = Some 1.
-Proof. reflexivity. Qed.
-Example test_update_5: (idUpdate (Id "y") 2 (idUpdate (Id "x") 1 idEmpty) (Id "y")) = Some 2.
-Proof. reflexivity. Qed.
-
 
 (** types **)
 
 Inductive T : Type :=
-  | Arrow  : T -> T -> T
-  | Unit   : T
+  | Arrow : T -> T -> T
+  | Unit : T
   | Option : T -> T
-  | List   : T -> T
+  | List : T -> T
   | Remote : P -> T
   | Signal : T -> T
-  | Var    : T -> T
-  | Tnat   : T.
+  | Var : T -> T
+  | Tnat : T.
 
 Notation "T1 ~> T2" := (Arrow T1 T2) (at level 30, right associativity).
-
-Fixpoint beq_T (a b: T): bool :=
-  match (a, b) with
-  | (a1 ~> a2, b1 ~> b2) => (beq_T a1 b1) && (beq_T a2 b2)
-  | (Unit, Unit) => true
-  | (Option a1, Option b1) => beq_T a1 b1
-  | (List a1, List b1) => beq_T a1 b1
-  | (Remote Pa, Remote Pb) => if peer_dec Pa Pb then true else false
-  | (Signal a1, Signal b1) => beq_T a1 b1
-  | (Var a1, Var b1) => beq_T a1 b1
-  | _ => false
-  end.
 
 
 (** placement types **)
@@ -95,82 +69,53 @@ Inductive S : Type :=
 
 Infix "on" := on (at level 20).
 
-Definition beq_S (a b: S): bool :=
-  match (a, b) with
-  | (aT on aP, bT on bP) => (beq_T aT bT) && (if peer_dec aP bP then true else false)
-  end.
 
 (** terms **)
 
 Inductive t : Type := 
   | lambda : id -> T -> t -> t
-  | app    : t -> t -> t
-  | idApp  : id -> t
-  | unit   : t
-  | none   : T -> t
-  | some   : t -> t
-  | nil    : T -> t
-  | cons   : t -> t -> t
-  | asLocal       : t -> S -> t 
-  | asLocalFrom   : t -> S -> t -> t
-  | asLocalIn     : id -> T -> t -> t -> S -> t
+  | app : t -> t -> t
+  | idApp : id -> t
+  | unit : t
+  | none : T -> t
+  | some : t -> t
+  | nil : T -> t
+  | cons : t -> t -> t
+  | asLocal : t -> S -> t 
+  | asLocalFrom : t -> S -> t -> t
+  | asLocalIn : id -> T -> t -> t -> S -> t
   | asLocalInFrom : id -> T -> t -> t -> S -> t -> t
   | signal : t -> t
-  | var    : t -> t
-  | now    : t -> t
-  | set    : t -> t -> t
-  | peerApp  : (ListSet.set p) -> t
+  | var : t -> t
+  | now : t -> t
+  | set : t -> t -> t
+  | peerApp : (ListSet.set p) -> t
   | reactApp : r -> t
-  | tnat     : nat -> t.
+  | tnat : nat -> t.
 
-(*
-Notation "\ x ; T , t" := (lambda (Id x) T t) (at level 80, left associativity).
-Example testNotationLambda1: (\ "z" ; Unit , unit) = (lambda (Id "z") Unit unit).
-Proof. reflexivity. Qed.
-*)
 
-Fixpoint beq_t (a b: t): bool :=
-  match (a, b) with
-  | (lambda ax aT at_, lambda bx bT bt)
-      => (if id_dec ax bx then true else false) && (beq_T aT bT) && (beq_t at_ bt)
-  | (app at1 at2, app bt1 bt2)    => (beq_t at1 bt1) && (beq_t at2 bt2)
-  | (idApp xa, idApp xb)          => if id_dec xa xb then true else false
-  | (unit, unit)                  => true
-  | (none aT, none bT)            => beq_T aT bT
-  | (some at1, some bt1)          => beq_t at1 bt1
-  | (nil aT, nil bT)              => beq_T aT bT
-  | (cons at1 at2, cons bt1 bt2)  => (beq_t at1 bt1) && (beq_t at2 bt2)
-  | (asLocal at1 aS, asLocal bt1 bS) 
-      => (beq_t at1 bt1) && (beq_S aS bS)
-  | (asLocalFrom at1 aS at2, asLocalFrom bt1 bS bt2)
-      => (beq_t at1 bt1) && (beq_S aS bS) && (beq_t at2 bt2)
-  | (asLocalIn ax aT at1 at2 aS, asLocalIn bx bT bt1 bt2 bS)
-      => (if id_dec ax bx then true else false) && (beq_T aT bT) && (beq_t at1 at2) && (beq_t at2 bt2) && (beq_S aS bS)
-  | (asLocalInFrom ax aT at1 at2 aS at3, asLocalInFrom bx bT bt1 bt2 bS bt3)
-      => (if id_dec ax bx then true else false) && (beq_T aT bT) && (beq_t at1 at2) && (beq_t at2 bt2) && (beq_S aS bS) && (beq_t at3 bt3)
-  | (signal at1, signal bt1)      => beq_t at1 bt1
-  | (var at1, var bt1)            => beq_t at1 bt1
-  | (now at1, now bt1)            => beq_t at1 bt1
-  | (set at1 at2, set bt1 bt2)    => (beq_t at1 bt1) && (beq_t at2 bt2)
-  | (peerApp ap, peerApp bp)      => (Nat.eqb (List.length ap) (List.length bp)) && (Nat.eqb (List.length ap) (List.length (ListSet.set_union peer_instance_dec ap bp)))
-  | (reactApp ar, reactApp br)    => if reactive_dec ar br then true else false
-  | (tnat an, tnat bn)            => Nat.eqb an bn
-  | _                             => false
-  end.
+(** placed terms **)
+
+Inductive s : Type :=
+  | placed : id -> S -> t -> s -> s
+  | pUnit  : s.
 
 
 (** values **)
 
-Inductive value : t -> Prop :=
-  | v_lambda : forall x T t, value (lambda x T t)
-  | v_unit : value unit
-  | v_none : forall T, value (none T)
-  | v_some : forall t, value t -> value (some t)
-  | v_nil : forall T, value (nil T)
-  | v_cons : forall t0 t1, value t0 -> value t1 -> value (cons t0 t1)
-  | v_peerApp : forall p, value (peerApp p)
-  | v_reactApp : forall r, value (reactApp r)
-  | v_tnat : forall n, value (tnat n).
+Inductive value_t : t -> Prop :=
+  | v_lambda : forall x T t, value_t (lambda x T t)
+  | v_unit : value_t unit
+  | v_none : forall T, value_t (none T)
+  | v_some : forall t, value_t t -> value_t (some t)
+  | v_nil : forall T, value_t (nil T)
+  | v_cons : forall t0 t1, value_t t0 -> value_t t1 -> value_t (cons t0 t1)
+  | v_peerApp : forall p, value_t (peerApp p)
+  | v_reactApp : forall r, value_t (reactApp r)
+  | v_tnat : forall n, value_t (tnat n).
+
+Inductive value_s : s -> Prop :=
+  | v_pUnit : value_s pUnit.
 
 Inductive transmittable_type : T -> Prop :=
   | U_Unit : transmittable_type Unit
@@ -180,12 +125,6 @@ Inductive transmittable_type : T -> Prop :=
   | U_Signal : forall T, transmittable_type T -> transmittable_type (Signal T)
   | U_Tnat : transmittable_type Tnat.
 
-
-(** placed terms **)
-
-Inductive s : Type :=
-  | placed : id -> S -> t -> s -> s
-  | pUnit  : s.
 
 
 (** ties **)
@@ -199,15 +138,6 @@ Notation "P1 -?-> P2" := (Tie (Peer P1) (Peer P2) Optional) (at level 20).
 Notation "P1 -1-> P2" := (Tie (Peer P1) (Peer P2) Single) (at level 20).
 Notation "P1 -0-> P2" := (Tie (Peer P1) (Peer P2) None) (at level 20).
 
-Example testNotation_multipleTie: "x" -*-> "y" = Tie (Peer "x") (Peer "y") Multiple.
-Proof. reflexivity. Qed.
-Example testNotation_optionalTie: "x" -?-> "y" = Tie (Peer "x") (Peer "y") Optional.
-Proof. reflexivity. Qed.
-Example testNotation_singleTie: "x" -1-> "y" = Tie (Peer "x") (Peer "y") Single.
-Proof. reflexivity. Qed.
-Example testNotation_noneTie: "x" -0-> "y" = Tie (Peer "x") (Peer "y") None.
-Proof. reflexivity. Qed.
-
 Definition ties := total_map (P * P) multiplicity.
 
 Definition NoTies: ties := t_empty None.
@@ -218,12 +148,6 @@ Definition ties_add (new_tie: tie) (current_ties: ties): ties :=
       if peer_dec x1 y1 then if peer_dec x2 y2 then true else false else false
     end) current_ties (p1, p2) mult
   end.
-
-Example test_tiesAdd_1: (ties_add ("x" -1-> "y") NoTies) (Peer "x", Peer "y") = Single.
-Proof. reflexivity. Qed.
-
-Example test_tiesAdd_2: (ties_add ("x" -1-> "y") NoTies) (Peer "y", Peer "x") = None.
-Proof. reflexivity. Qed.
 
 Notation "'Ties' [ ]" := NoTies (at level 50).
 
@@ -278,13 +202,6 @@ Fixpoint typed_peer_instances_of_type
       else typed_peer_instances_of_type instances P
   end.
 
-Example test_typedPeerInstancesAdd_1: typed_peer_instances_type
-                                        (typed_peer_instances_add (PeerInstance 1, Peer "x")
-                                          (typed_peer_instances_add (PeerInstance 2, Peer "y")
-                                            NoTypedInstances))
-                                        (PeerInstance 2) = Some (Peer "y").
-Proof. reflexivity. Qed.
-
 Notation "p : P" := (PeerInstance p, Peer P) (at level 40).
 
 Notation "'TypedInstances' [ ]" := NoTypedInstances (at level 50).
@@ -328,6 +245,87 @@ Definition peer_instances_of_type program P: ListSet.set p :=
 
 Definition peers_tied program P0 P1: Prop :=
   (peer_ties program) (P0, P1) <> None /\ (peer_ties program) (P1, P0) <> None.
+
+Definition is_remote_subterm subterm term : Prop :=
+  match term with
+  | lambda x type t => False
+  | app t0 t1 => False
+  | idApp _x => False
+  | unit => False
+  | none type => False
+  | some t => False
+  | nil type => False
+  | cons t0 t1 => False
+  | asLocal t type => t = subterm
+  | asLocalFrom t0 type t1 => t0 = subterm
+  | asLocalIn x' type0 t0 t1 type1 => t1 = subterm
+  | asLocalInFrom x' type0 t0 t1 type1 t2 => t1 = subterm
+  | signal t => False
+  | var t => False
+  | now t => False
+  | set t0 t1 => False
+  | peerApp peer => False
+  | reactApp reactive => False
+  | tnat n => False
+  end.
+
+Definition is_reducing_subterm_t subterm term : Prop :=
+  match term with
+  | lambda x type t => False
+  | app t0 t1 => t0 = subterm /\ ~ value_t t0 \/ t1 = subterm /\ ~ value_t t1 /\ value_t t0
+  | idApp _x => False
+  | unit => False
+  | none type => False
+  | some t => t = subterm /\ ~ value_t t
+  | nil type => False
+  | cons t0 t1 => t0 = subterm /\ ~ value_t t0 \/ t1 = subterm /\ ~ value_t t1 /\ value_t t0
+  | asLocal t type => t = subterm /\ ~ value_t t
+  | asLocalFrom t0 type t1 => t0 = subterm /\ ~ value_t t0 /\ value_t t1 \/ t1 = subterm /\ ~ value_t t1
+  | asLocalIn x' type0 t0 t1 type1 => t0 = subterm /\ ~ value_t t0
+  | asLocalInFrom x' type0 t0 t1 type1 t2 => t0 = subterm /\ ~ value_t t0 /\ value_t t2 \/ t2 = subterm /\ ~ value_t t2
+  | signal t => False
+  | var t => t = subterm /\ ~ value_t t
+  | now t => t = subterm /\ ~ value_t t
+  | set t0 t1 => t0 = subterm /\ ~ value_t t0 \/ t1 = subterm /\ ~ value_t t1 /\ value_t t0
+  | peerApp peer => False
+  | reactApp reactive => False
+  | tnat n => False
+  end.
+
+Definition is_reducing_subterm_s subterm term : Prop :=
+  match term with
+  | placed x type t s => t = subterm /\ ~ value_t t
+  | pUnit => False
+  end.
+
+Definition is_subterm_t subterm term : Prop :=
+  match term with
+  | lambda x type t => t = subterm
+  | app t0 t1 => t0 = subterm \/ t1 = subterm
+  | idApp _x => False
+  | unit => False
+  | none type => False
+  | some t => t = subterm
+  | nil type => False
+  | cons t0 t1 => t0 = subterm \/ t1 = subterm
+  | asLocal t type => t = subterm
+  | asLocalFrom t0 type t1 => t0 = subterm \/ t1 = subterm
+  | asLocalIn x' type0 t0 t1 type1 => t0 = subterm \/ t1 = subterm
+  | asLocalInFrom x' type0 t0 t1 type1 t2 => t0 = subterm \/ t1 = subterm \/ t2 = subterm
+  | signal t => t = subterm
+  | var t => t = subterm
+  | now t => t = subterm
+  | set t0 t1 => t0 = subterm \/ t1 = subterm
+  | peerApp peer => False
+  | reactApp reactive => False
+  | tnat n => False
+  end.
+
+Definition is_subterm_s subterm term : Prop :=
+  match term with
+  | placed x type t s => t = subterm
+  | pUnit => False
+  end.
 
 
 Inductive var_locality : Type := LocalOrRemoteVar | RemoteVar.
