ProofExplicitRemoteAccess.v
@@ -1,0 +1,86 @@
+Require Import Syntax.
+Require Import SemanticsStatic.
+
+Lemma explicit_remote_access: forall t t' T program Psi Delta Gamma P,
+  program :: Psi; Delta; Gamma; P |- t : T ->
+  is_subterm_t t' t ->
+  exists T' Psi' Delta' Gamma' P',
+   program :: Psi'; Delta'; Gamma'; P' |- t' : T' /\
+   (is_remote_subterm t' t \/ P' = P).
+Proof.
+intros until P.
+pose (term := t).
+intros H_typing H_subterm.
+destruct H_typing; simpl in H_subterm; subst.
+- contradiction.
+- destruct H_subterm as [ H_subterm | H_subterm ]; subst.
+  + exists (T2 ~> T1), Psi, Delta, Gamma, P.
+    split; try assumption.
+    right. reflexivity.
+  + exists T2, Psi, Delta, Gamma, P.
+    split; try assumption.
+    right. reflexivity.
+- exists T2, Psi, Delta, (idUpdate x T1 Gamma), P.
+  split; try assumption.
+  right. reflexivity.
+- destruct H_subterm as [ H_subterm | H_subterm ]; subst.
+  + exists T, Psi, Delta, Gamma, P.
+    split; try assumption.
+    right. reflexivity.
+  + exists (List T), Psi, Delta, Gamma, P.
+    split; try assumption.
+    right. reflexivity.
+- contradiction.
+- exists T, Psi, Delta, Gamma, P.
+  split; try assumption.
+  right. reflexivity.
+- contradiction.
+- contradiction.
+- contradiction.
+- exists T1, Psi, Delta, emptyVarEnv, P1.
+  split; try assumption.
+  left. reflexivity.
+- destruct H_subterm as [ H_subterm | H_subterm ]; subst.
+  + exists T, Psi, Delta, emptyVarEnv, P1.
+    split; try assumption.
+    left. reflexivity.
+  + exists (Remote P1), Psi, Delta, Gamma, P0.
+    split; try assumption.
+    right. reflexivity.
+- destruct H_subterm as [ H_subterm | H_subterm ]; subst.
+  + exists T0, Psi, Delta, Gamma, P0.
+    split; try assumption.
+    right. reflexivity.
+  + exists T1, Psi, Delta, (idUpdate x T0 emptyVarEnv), P1.
+    split; try assumption.
+    left. reflexivity.
+- destruct H_subterm as [ H_subterm | H_subterm ]; subst.
+  + exists T0, Psi, Delta, Gamma, P0.
+    split; try assumption.
+    right. reflexivity.
+  + destruct H_subterm as [ H_subterm | H_subterm ]; subst.
+    * exists T1, Psi, Delta, (idUpdate x T0 emptyVarEnv), P1.
+      split; try assumption.
+      left. reflexivity.
+    * exists (Remote P1), Psi, Delta, Gamma, P0.
+      split; try assumption.
+      right. reflexivity.
+- contradiction.
+- exists T, Psi, Delta, Gamma, P.
+  split; try assumption.
+  right. reflexivity.
+- exists T, Psi, Delta, Gamma, P.
+  split; try assumption.
+  right. reflexivity.
+- exists T0, Psi, Delta, Gamma, P.
+  split; try assumption.
+  right. reflexivity.
+- destruct H_subterm as [ H_subterm | H_subterm ]; subst.
+  + exists (Var T), Psi, Delta, Gamma, P.
+    split; try assumption.
+    right. reflexivity.
+  + exists T, Psi, Delta, Gamma, P.
+    split; try assumption.
+    right. reflexivity.
+- contradiction.
+Qed.
