ProofPreservation.v
@@ -1,0 +1,284 @@
+Require Import Syntax.
+Require Import SemanticsStatic.
+Require Import SemanticsDynamic.
+Require Import ProofContext.
+Require Import ProofSubstitution.
+Require Import ProofReactiveSystem.
+Require Import ProofTransmission.
+Require Import ProofAggregation.
+
+Theorem preservation_t: forall t t' T theta theta' program Psi P rho rho',
+  program :: Psi; emptyPlaceEnv; emptyVarEnv; P |- t : T ->
+  program :: Psi; emptyPlaceEnv; emptyVarEnv |- rho ->
+  List.incl theta (peer_instances_of_type program P) ->
+  program :: theta : P |> t; rho == theta' ==> t'; rho' ->
+  exists Psi',
+    Psi' extends Psi /\
+    program :: Psi'; emptyPlaceEnv; emptyVarEnv; P |- t' : T /\
+    program :: Psi'; emptyPlaceEnv; emptyVarEnv |- rho'.
+Proof.
+intros until rho'.
+intros H_typing H_reactive_typing H_instances H_eval.
+remember emptyPlaceEnv as Delta.
+remember emptyVarEnv as Gamma.
+generalize dependent theta.
+generalize dependent t'.
+induction H_typing; intros; subst.
+- inversion H_eval.
+- inversion H_eval; subst.
+  + apply IHH_typing1 in H8; try assumption || reflexivity.
+    destruct H8 as [ Psi' ].
+    destruct H, H0.
+    exists Psi'.
+    do 2 (split; try assumption).
+    eapply T_App; try eassumption.
+    eapply reactive_typing_weakening_t; eassumption.
+  + apply IHH_typing2 in H9; try assumption || reflexivity.
+    destruct H9 as [ Psi' ].
+    destruct H, H0.
+    exists Psi'.
+    do 2 (split; try assumption).
+    eapply T_App; try eassumption.
+    eapply reactive_typing_weakening_t; eassumption.
+  + inversion H_typing1.
+    subst.
+    exists Psi.
+    split.
+    * apply reactive_typing_extends_refl.
+    * split; try assumption.
+      eapply substitution_t; eassumption.
+- inversion H_eval.
+- inversion H_eval; subst.
+  + apply IHH_typing1 in H8; try assumption || reflexivity.
+    destruct H8 as [ Psi' ].
+    destruct H, H0.
+    exists Psi'.
+    do 2 (split; try assumption).
+    eapply T_Cons; try eassumption.
+    eapply reactive_typing_weakening_t; eassumption.
+  + apply IHH_typing2 in H9; try assumption || reflexivity.
+    destruct H9 as [ Psi' ].
+    destruct H, H0.
+    exists Psi'.
+    do 2 (split; try assumption).
+    eapply T_Cons; try eassumption.
+    eapply reactive_typing_weakening_t; eassumption.
+- inversion H_eval.
+- inversion H_eval; subst.
+  apply IHH_typing in H3; try assumption || reflexivity.
+  destruct H3 as [ Psi' ].
+  destruct H, H0.
+  exists Psi'.
+  do 2 (split; try assumption).
+  eapply T_Some; try eassumption.
+- inversion H_eval.
+- inversion H_eval.
+- inversion H_eval.
+- inversion H_eval; subst.
+  + exists Psi.
+    split.
+    * apply reactive_typing_extends_refl.
+    * split; try assumption.
+      eapply aggregation; try eassumption.
+      apply List.incl_refl.
+  + apply IHH_typing in H12; try assumption || reflexivity.
+    * destruct H12 as [ Psi' ].
+      destruct H2, H3.
+      exists Psi'.
+      do 2 (split; try assumption).
+      eapply T_AsLocal; try eassumption.
+    * apply List.incl_refl.
+- inversion H_eval; subst.
+  + apply IHH_typing2 in H11; try assumption || reflexivity.
+    destruct H11 as [ Psi' ].
+    destruct H1, H2.
+    exists Psi'.
+    do 2 (split; try assumption).
+    eapply T_AsLocalFrom; try eassumption.
+    eapply reactive_typing_weakening_t; eassumption.
+  + inversion H_typing2.
+    subst.
+    exists Psi.
+    split.
+    * apply reactive_typing_extends_refl.
+    * split; try assumption.
+      eapply transmission; try eassumption.
+  + inversion H_typing2.
+    subst.
+    apply IHH_typing1 in H12; try assumption || reflexivity.
+    destruct H12 as [ Psi' ].
+    destruct H1, H2.
+    exists Psi'.
+    do 2 (split; try assumption).
+    eapply T_AsLocalFrom; try eassumption.
+    eapply reactive_typing_weakening_t; eassumption.
+- inversion H_eval; subst.
+  + apply IHH_typing1 in H15; try assumption || reflexivity.
+    destruct H15 as [ Psi' ].
+    destruct H3, H4.
+    exists Psi'.
+    do 2 (split; try assumption).
+    eapply T_Comp; try eassumption.
+    eapply reactive_typing_weakening_t; eassumption.
+  + exists Psi.
+    split.
+    * apply reactive_typing_extends_refl.
+    * split; try assumption.
+      eapply T_AsLocal; try eassumption.
+      eapply substitution_t; try eassumption.
+      eapply transmission; try eassumption.
+      unfold peers_tied in H1.
+      destruct H1.
+      unfold peers_tied.
+      split; assumption.
+- inversion H_eval; subst.
+  + apply IHH_typing3 in H15; try assumption || reflexivity.
+    destruct H15 as [ Psi' ].
+    destruct H2, H3.
+    exists Psi'.
+    do 2 (split; try assumption).
+    eapply T_ComFrom; try eassumption.
+    * eapply reactive_typing_weakening_t; eassumption.
+    * eapply reactive_typing_weakening_t; eassumption.
+  + apply IHH_typing1 in H16; try assumption || reflexivity.
+    destruct H16 as [ Psi' ].
+    destruct H2, H3.
+    exists Psi'.
+    do 2 (split; try assumption).
+    eapply T_ComFrom; try eassumption.
+    * eapply reactive_typing_weakening_t; eassumption.
+    * eapply reactive_typing_weakening_t; eassumption.
+  + exists Psi.
+    split.
+    * apply reactive_typing_extends_refl.
+    * split; try assumption.
+      eapply T_AsLocalFrom; try eassumption.
+      eapply substitution_t; try eassumption.
+      eapply transmission; try eassumption.
+      unfold peers_tied in H1.
+      destruct H1.
+      unfold peers_tied.
+      split; assumption.
+- inversion H_eval.
+- inversion H_eval.
+  subst.
+  pose proof reactive_typing_add.
+  specialize H with program Psi emptyPlaceEnv emptyVarEnv rho P t T (Signal T).
+  apply H in H_reactive_typing as H0; try assumption || (right; reflexivity).
+  destruct H0 as [ Psi' ], H0 as [ rho0 ], H0 as [ r' ].
+  destruct H0, H1, H2, H4.
+  rewrite H3 in H1.
+  inversion H1.
+  subst.
+  exists Psi'.
+  do 2 (split; try assumption).
+  eapply T_Reactive; try eassumption.
+  left. reflexivity.
+- inversion H_eval; subst.
+  + apply IHH_typing in H3; try assumption || reflexivity.
+    destruct H3 as [ Psi' ].
+    destruct H, H0.
+    exists Psi'.
+    do 2 (split; try assumption).
+    apply T_ReactiveVar.
+    eapply reactive_typing_weakening_t; eassumption.
+  + pose proof reactive_typing_add.
+    specialize H with program Psi emptyPlaceEnv emptyVarEnv rho P t T (Var T).
+    apply H in H_reactive_typing as H1; try assumption || (left; reflexivity).
+    destruct H1 as [ Psi' ], H1 as [ rho0 ], H1 as [ r' ].
+    destruct H1, H2, H3, H5.
+    rewrite H4 in H2.
+    inversion H2.
+    subst.
+    exists Psi'.
+    do 2 (split; try assumption).
+    eapply T_Reactive; try eassumption.
+    right. reflexivity.
+- inversion H_eval; subst.
+  + apply IHH_typing in H4; try assumption || reflexivity.
+    destruct H4 as [ Psi' ].
+    destruct H0, H1.
+    exists Psi'.
+    do 2 (split; try assumption).
+    eapply T_Now; try eassumption.
+    eapply reactive_typing_weakening_t; eassumption.
+  + inversion H_typing.
+    subst.
+    exists Psi.
+    split.
+    * apply reactive_typing_extends_refl.
+    * { split; try assumption.
+        unfold reactive_system_well_typed in H_reactive_typing.
+        destruct H_reactive_typing as [ H0 H2 ].
+        specialize H2 with r.
+        assert (reactive_system_lookup r rho' <> Datatypes.None).
+        - congruence.
+        - apply reactive_system_lookup_domain in H3.
+          apply H2 in H3.
+          destruct H3 as [ t2 ], H3 as [ T2 ], H3 as [ T2' ], H3 as [ P2 ].
+          destruct H3, H5, H6.
+          rewrite H4 in H3.
+          inversion H3.
+          rewrite H1 in H5.
+          inversion H5.
+          destruct H, H6; subst; congruence.
+      }
+- inversion H_eval; subst.
+  + apply IHH_typing1 in H8; try assumption || reflexivity.
+    destruct H8 as [ Psi' ].
+    destruct H, H0.
+    exists Psi'.
+    do 2 (split; try assumption).
+    eapply T_Set; try eassumption.
+    eapply reactive_typing_weakening_t; eassumption.
+  + apply IHH_typing2 in H9; try assumption || reflexivity.
+    destruct H9 as [ Psi' ].
+    destruct H, H0.
+    exists Psi'.
+    do 2 (split; try assumption).
+    eapply T_Set; try eassumption.
+    eapply reactive_typing_weakening_t; eassumption.
+  + inversion H_typing1.
+    subst.
+    pose proof reactive_typing_update.
+    specialize H with program Psi emptyPlaceEnv emptyVarEnv rho r P t2 T.
+    apply H in H_reactive_typing as H1; try assumption.
+    exists Psi.
+    split.
+    * apply reactive_typing_extends_refl.
+    * split; try assumption.
+      apply T_Unit.
+- inversion H_eval.
+Qed.
+
+
+Theorem preservation_s: forall s s' theta program Psi rho rho',
+  program :: Psi; emptyPlaceEnv |- s ->
+  program :: Psi; emptyPlaceEnv; emptyVarEnv |- rho ->
+  program :: s; rho == theta ==> s'; rho' ->
+  exists Psi',
+    Psi' extends Psi /\
+    program :: Psi'; emptyPlaceEnv |- s' /\
+    program :: Psi'; emptyPlaceEnv; emptyVarEnv |- rho'.
+Proof.
+intros until rho'.
+intros H_typing H_reactive_typing H_eval.
+remember emptyPlaceEnv as Delta.
+generalize dependent s'.
+destruct H_typing; intros; subst.
+- inversion H_eval.
+- inversion H_eval; subst.
+  + eapply preservation_t in H10; try eassumption.
+    * destruct H10 as [ Psi' ].
+      destruct H0, H1.
+      exists Psi'.
+      do 2 (split; try assumption).
+      apply T_Place; try assumption.
+      eapply reactive_typing_weakening_s; eassumption.
+    * apply List.incl_refl.
+  + exists Psi.
+    split.
+    * apply reactive_typing_extends_refl.
+    * split; try assumption.
+      eapply substitution_s; eassumption.
+Qed.
