ProofProgress.v
@@ -1,0 +1,223 @@
+Require Import Syntax.
+Require Import SemanticsStatic.
+Require Import SemanticsDynamic.
+Require Import ProofReactiveSystem.
+
+
+Definition config_complete program :=
+  forall P0 P1,
+  ((peer_ties program) (P0, P1) = Single ->
+   length (peer_instances_of_type program P1) = 1) /\
+  ((peer_ties program) (P0, P1) = Optional ->
+   length (peer_instances_of_type program P1) <= 1).
+
+
+Lemma some_phi: forall program t T P0 P1,
+  config_complete program ->
+  peers_tied program P0 P1 ->
+  exists t', Phi (peer_ties program) P0 P1 (peer_instances_of_type program P1) t T = Some t'.
+Proof.
+intros until P1.
+intros H_complete H_tied.
+destruct program as [ ties peers ].
+unfold peers_tied in H_tied.
+destruct H_tied as [ H_P0_tied H_P1_tied ].
+simpl in H_P0_tied.
+clear H_P1_tied.
+unfold config_complete, peer_ties in H_complete.
+destruct (ties (P0, P1)) eqn: H_tie.
+- clear H_complete.
+  induction (peer_instances_of_type (Program ties peers) P1) as [| p peers' IH_peers ].
+  + simpl.
+    rewrite H_tie.
+    esplit.
+    reflexivity.
+  + simpl.
+    rewrite H_tie.
+    destruct IH_peers.
+    simpl in H.
+    rewrite H.
+    esplit.
+    reflexivity.
+- apply H_complete in H_tie as H_peers_length.
+  destruct (peer_instances_of_type (Program ties peers) P1) as [| p peers' ].
+  + simpl.
+    rewrite H_tie.
+    esplit.
+    reflexivity.
+  + destruct peers'.
+    * simpl.
+      rewrite H_tie.
+      esplit.
+      reflexivity.
+    * simpl in H_peers_length.
+      apply le_S_n in H_peers_length.
+      inversion H_peers_length.
+- apply H_complete in H_tie as H_peers_length.
+  destruct (peer_instances_of_type (Program ties peers) P1) as [| p peers' ].
+  + inversion H_peers_length.
+  + destruct peers'.
+    * simpl.
+      rewrite H_tie.
+      esplit.
+      reflexivity.
+    * simpl in H_peers_length.
+      congruence.
+- congruence.
+Qed.
+
+
+Theorem progress_t: forall t T theta program Psi P rho,
+  config_complete program ->
+  program :: Psi; emptyPlaceEnv; emptyVarEnv; P |- t : T ->
+  program :: Psi; emptyPlaceEnv; emptyVarEnv |- rho ->
+  value_t t \/ exists t' theta' rho', program :: theta : P |> t; rho == theta' ==> t'; rho'.
+Proof.
+intros until rho.
+intros H_complete H_typing H_reactive_typing.
+remember emptyPlaceEnv as Delta.
+remember emptyVarEnv as Gamma.
+generalize dependent theta.
+induction H_typing; intros; subst.
+- destruct H.
+  + unfold emptyVarEnv, idEmpty, Maps.p_empty in H.
+    congruence.
+  + destruct H.
+    unfold emptyPlaceEnv, idEmpty, Maps.p_empty in H0.
+    congruence.
+- edestruct IHH_typing1; try assumption || reflexivity.
+  + edestruct IHH_typing2; try assumption || reflexivity.
+    * { inversion H; subst; inversion H_typing1; subst.
+        - right. repeat esplit.
+          apply E_App. assumption.
+        - destruct H8; congruence.
+      }
+    * destruct H0 as [ t2' ], H0 as [ theta' ], H0 as [ rho' ].
+      right. repeat esplit.
+      apply EC_App_Right; eassumption.
+  + destruct H as [ t1' ], H as [ theta' ], H as [ rho' ].
+    right. repeat esplit.
+    apply EC_App_Left. eassumption.
+- left. apply v_lambda.
+- edestruct IHH_typing1; try assumption || reflexivity.
+  + edestruct IHH_typing2; try assumption || reflexivity.
+    * left. apply v_cons; assumption.
+    * destruct H0 as [ t1' ], H0 as [ theta' ], H0 as [ rho' ].
+      right. repeat esplit.
+      apply EC_Cons_Right; eassumption.
+  + destruct H as [ t0' ], H as [ theta' ], H as [ rho' ].
+    right. repeat esplit.
+    apply EC_Cons_Left. eassumption.
+- left. apply v_nil.
+- edestruct IHH_typing; try assumption || reflexivity.
+  + left. apply v_some. assumption.
+  + destruct H as [ t' ], H as [ theta' ], H as [ rho' ].
+    right. repeat esplit.
+    apply EC_Some. eassumption.
+- left. apply v_none.
+- left. apply v_unit.
+- left. apply v_peerApp.
+- edestruct IHH_typing; try assumption || reflexivity.
+  + pose proof some_phi.
+    eapply H3 in H0; try assumption.
+    destruct H0 as [ t' ].
+    right. repeat esplit.
+    eapply E_AsLocal; eassumption.
+  + destruct H2 as [ t' ], H2 as [ theta' ], H2 as [ rho' ].
+    right. repeat esplit.
+    apply E_Remote. eassumption.
+- edestruct IHH_typing2; try assumption || reflexivity.
+  + inversion H1; subst; inversion H_typing2; subst.
+    * { edestruct IHH_typing1; try assumption || reflexivity.
+        - right. repeat esplit.
+          apply E_AsLocalFrom; assumption || reflexivity.
+        - destruct H2 as [ t0' ], H2 as [ theta' ], H2 as [ rho' ].
+          right. repeat esplit.
+          apply E_RemoteFrom. eassumption.
+      }
+    * destruct H9; congruence.
+  + destruct H1 as [ t1' ], H1 as [ theta' ], H1 as [ rho' ].
+    right. repeat esplit.
+    apply EC_AsLocalFrom. eassumption.
+- edestruct IHH_typing1; try assumption || reflexivity.
+  + right. repeat esplit.
+    apply E_Comp; assumption || reflexivity.
+  + destruct H3 as [ t0' ], H3 as [ theta' ], H3 as [ rho' ].
+    right. repeat esplit.
+    apply EC_Comp. eassumption.
+- edestruct IHH_typing3; try assumption || reflexivity.
+  + inversion H2; subst; inversion H_typing3; subst.
+    * { edestruct IHH_typing1; try assumption || reflexivity.
+        - right. repeat esplit.
+          apply E_CompFrom; assumption || reflexivity.
+        - destruct H3 as [ t0' ], H3 as [ theta' ], H3 as [ rho' ].
+          right. repeat esplit.
+          apply EC_CompFrom_Left; eassumption.
+      }
+    * destruct H10; congruence.
+  + destruct H2 as [ t2' ], H2 as [ theta' ], H2 as [ rho' ].
+    right. repeat esplit.
+    apply EC_CompFrom_Right. eassumption.
+- left. apply v_reactApp.
+- right. repeat esplit.
+  eapply E_Signal.
+  reflexivity.
+- edestruct IHH_typing; try assumption || reflexivity.
+  + right. repeat esplit.
+    apply E_ReactiveVar; assumption || reflexivity.
+  + destruct H as [ t' ], H as [ theta' ], H as [ rho' ].
+    right. repeat esplit.
+    eapply EC_Var. eassumption.
+- edestruct IHH_typing; try assumption || reflexivity.
+  + inversion H0; subst; inversion H_typing; subst;
+      try solve [ destruct H; congruence ].
+    unfold reactive_system_well_typed in H_reactive_typing.
+    destruct H_reactive_typing as [ H1 H3 ].
+    specialize H3 with r.
+    assert (reactive_type r Psi <> Datatypes.None).
+    * congruence.
+    * apply reactive_env_type_domain in H4.
+      rewrite <- H1 in H4.
+      apply H3 in H4.
+      destruct H4 as [ t' ], H4 as [ T' ], H4 as [ T'' ], H4 as [ P' ], H4.
+      right. repeat esplit.
+      eapply E_Now. eassumption.
+  + destruct H0 as [ t' ], H0 as [ theta' ], H0 as [ rho' ].
+    right. repeat esplit.
+    eapply EC_Now. eassumption.
+- edestruct IHH_typing1; try assumption || reflexivity.
+  + edestruct IHH_typing2; try assumption || reflexivity.
+    * inversion H; subst; inversion H_typing1; subst.
+      right. repeat esplit.
+      eapply E_Set; assumption || reflexivity.
+    * destruct H0 as [ t2' ], H0 as [ theta' ], H0 as [ rho' ].
+      right. repeat esplit.
+      apply EC_Set_Right; eassumption.
+  + destruct H as [ t1' ], H as [ theta' ], H as [ rho' ].
+    right. repeat esplit.
+    apply EC_Set_Left. eassumption.
+- left. apply v_tnat.
+Qed.
+
+
+Theorem progress_s: forall s program Psi rho,
+  config_complete program ->
+  program :: Psi; emptyPlaceEnv |- s ->
+  program :: Psi; emptyPlaceEnv; emptyVarEnv |- rho ->
+  value_s s \/ exists s' theta rho', program :: s; rho == theta ==> s'; rho'.
+Proof.
+intros until rho.
+intros H_complete H_typing H_reactive_typing.
+remember emptyPlaceEnv as Delta.
+destruct H_typing; intros; subst.
+- left. apply v_pUnit.
+- eapply progress_t in H_complete; try eassumption.
+  destruct H_complete.
+  + right. repeat esplit.
+    apply E_Placed_Val.
+    assumption.
+  + destruct H0 as [ t' ], H0 as [ theta' ], H0 as [ rho' ].
+    right. repeat esplit.
+    eapply E_Placed.
+    eassumption.
+Qed.
