ProofStaticPlacement.v
@@ -1,0 +1,165 @@
+Require Import Syntax.
+Require Import SemanticsStatic.
+Require Import SemanticsDynamic.
+
+Lemma static_placement_t: forall t_i t t' T program Psi Delta Gamma P theta theta' rho rho',
+  program :: Psi; Delta; Gamma; P |- t : T ->
+  program :: theta : P |> t; rho == theta' ==> t'; rho' ->
+  List.incl theta (peer_instances_of_type program P) ->
+  is_reducing_subterm_t t_i t ->
+  (exists t_i' T_i Psi_i Delta_i Gamma_i P_i P_i' theta_i theta_i' rho_i rho_i',
+   program :: Psi_i; Delta_i; Gamma_i; P_i |- t_i : T_i /\
+   program :: theta_i : P_i' |> t_i; rho_i == theta_i' ==> t_i'; rho_i' /\
+   List.incl theta_i (peer_instances_of_type program P_i') /\
+   P_i = P_i').
+Proof.
+intros until rho'.
+intros H_typing H_eval H_subset H_subterm.
+assert (no_value_reduction:
+  forall t t' program P theta theta' rho rho',
+  program :: theta : P |> t; rho == theta' ==> t'; rho' -> ~ value_t t);
+  [ > intros; induction H; intro; solve [ inversion H0; contradiction | inversion H1; contradiction ] | ].
+destruct H_typing; simpl in H_subterm; subst.
+- contradiction.
+- destruct H_subterm as [ H_subterm | H_subterm ].
+  + destruct H_subterm as [ H_subterm H_subterm_no_value ].
+    inversion H_eval; subst.
+    * exists t0', (T2 ~> T1), Psi, Delta, Gamma, P, P, theta, theta', rho, rho'.
+      repeat split; reflexivity || assumption.
+    * contradiction.
+    * contradict H_subterm_no_value.
+      apply v_lambda.
+  + destruct
+      H_subterm as [ H_subterm H_subterm_value ],
+      H_subterm_value as [ H_subterm_no_value H_subterm_value ].
+    inversion H_eval; subst.
+    * apply no_value_reduction in H8.
+      contradiction.
+    * exists t1', T2, Psi, Delta, Gamma, P, P, theta, theta', rho, rho'.
+      repeat split; reflexivity || assumption.
+    * contradiction.
+- contradiction.
+- destruct H_subterm as [ H_subterm | H_subterm ].
+  + destruct H_subterm as [ H_subterm H_subterm_no_value ].
+    inversion H_eval; subst.
+    * exists t0', T, Psi, Delta, Gamma, P, P, theta, theta', rho, rho'.
+      repeat split; reflexivity || assumption.
+    * contradiction.
+  + destruct
+      H_subterm as [ H_subterm H_subterm_value ],
+      H_subterm_value as [ H_subterm_no_value H_subterm_value ].
+    inversion H_eval; subst.
+    * apply no_value_reduction in H8.
+      contradiction.
+    * exists t1', (List T), Psi, Delta, Gamma, P, P, theta, theta', rho, rho'.
+      repeat split; reflexivity || assumption.
+- contradiction.
+- destruct H_subterm.
+  inversion H_eval; subst.
+  exists t'0, T, Psi, Delta, Gamma, P, P, theta, theta', rho, rho'.
+  repeat split; reflexivity || assumption.
+- contradiction.
+- contradiction.
+- contradiction.
+- destruct H_subterm.
+  inversion H_eval; subst.
+  + contradiction.
+  + exists t'0, T1, Psi, Delta, emptyVarEnv, P1, P1, (peer_instances_of_type program P1), theta', rho, rho'.
+    repeat split; try reflexivity || assumption.
+    apply List.incl_refl.
+- destruct H_subterm as [ H_subterm | H_subterm ].
+  + destruct
+      H_subterm as [ H_subterm H_subterm_value ],
+      H_subterm_value as [ H_subterm_no_value H_subterm_value ].
+    inversion H_eval; subst.
+    * apply no_value_reduction in H11.
+      contradiction.
+    * contradiction.
+    * exists t'0, T, Psi, Delta, emptyVarEnv, P1, P1, theta'', theta', rho, rho'.
+      inversion H_typing2.
+      repeat split; try reflexivity || assumption.
+  + destruct H_subterm as [ H_subterm H_subterm_no_value ].
+    inversion H_eval; subst.
+    * exists t1', (Remote P1), Psi, Delta, Gamma, P0, P0, theta, theta', rho, rho'.
+      repeat split; reflexivity || assumption.
+    * contradict H_subterm_no_value.
+      apply v_peerApp.
+    * contradict H_subterm_no_value.
+      apply v_peerApp.
+- destruct H_subterm as [ H_subterm H_subterm_no_value ].
+  inversion H_eval; subst.
+  + exists t0', T0, Psi, Delta, Gamma, P0, P0, theta, theta', rho, rho'.
+    repeat split; reflexivity || assumption.
+  + contradiction.
+- destruct H_subterm as [ H_subterm | H_subterm ].
+  + destruct
+      H_subterm as [ H_subterm H_subterm_value ],
+      H_subterm_value as [ H_subterm_no_value H_subterm_value ].
+    inversion H_eval; subst.
+    * apply no_value_reduction in H15.
+      contradiction.
+    * exists t0', T0, Psi, Delta, Gamma, P0, P0, theta, theta', rho, rho'.
+      repeat split; reflexivity || assumption.
+    * contradiction.
+  + destruct H_subterm as [ H_subterm H_subterm_no_value ].
+    inversion H_eval; subst.
+    * exists t2', (Remote P1), Psi, Delta, Gamma, P0, P0, theta, theta', rho, rho'.
+      repeat split; reflexivity || assumption.
+    * contradiction.
+    * contradict H_subterm_no_value.
+      apply v_peerApp.
+- contradiction.
+- contradiction.
+- destruct H_subterm.
+  inversion H_eval; subst.
+  * exists t'0, T, Psi, Delta, Gamma, P, P, theta, theta', rho, rho'.
+    repeat split; reflexivity || assumption.
+  * contradiction.
+- destruct H_subterm.
+  inversion H_eval; subst.
+  * exists t'0, T0, Psi, Delta, Gamma, P, P, theta, theta', rho, rho'.
+    repeat split; reflexivity || assumption.
+  * contradict H1.
+    apply v_reactApp.
+- destruct H_subterm as [ H_subterm | H_subterm ].
+  + destruct H_subterm as [ H_subterm H_subterm_no_value ].
+    inversion H_eval; subst.
+    * exists t0', (Var T), Psi, Delta, Gamma, P, P, theta, theta', rho, rho'.
+      repeat split; reflexivity || assumption.
+    * contradiction.
+    * contradict H_subterm_no_value.
+      apply v_reactApp.
+  + destruct
+      H_subterm as [ H_subterm H_subterm_value ],
+      H_subterm_value as [ H_subterm_no_value H_subterm_value ].
+    inversion H_eval; subst.
+    * apply no_value_reduction in H8.
+      contradiction.
+    * exists t1', T, Psi, Delta, Gamma, P, P, theta, theta', rho, rho'.
+      repeat split; reflexivity || assumption.
+    * contradiction.
+- contradiction.
+Qed.
+
+
+Lemma static_placement_s: forall t_i s s' program Psi Delta theta rho rho',
+  program :: Psi; Delta |- s ->
+  program :: s; rho == theta ==> s'; rho' ->
+  is_reducing_subterm_s t_i s ->
+  (exists t_i' T_i Psi_i Delta_i Gamma_i P_i P_i' theta_i theta_i' rho_i rho_i',
+   program :: Psi_i; Delta_i; Gamma_i; P_i |- t_i : T_i /\
+   program :: theta_i : P_i' |> t_i; rho_i == theta_i' ==> t_i'; rho_i' /\
+   List.incl theta_i (peer_instances_of_type program P_i') /\
+   P_i = P_i').
+Proof.
+intros until rho'.
+intros H_typing H_eval H_subterm.
+destruct H_typing; simpl in H_subterm; subst.
+- contradiction.
+- destruct H_subterm as [ H_subterm H_subterm_no_value ].
+  inversion H_eval; subst.
+  + exists t', T, Psi, Delta, emptyVarEnv, P, P, (peer_instances_of_type program P), theta, rho, rho'.
+    repeat split; try reflexivity || assumption.
+    apply List.incl_refl.
+  + contradiction.
+Qed.
