ReTierProofPeerTies.v
@@ -1,9 +1,0 @@
-Require Import ReTierSyntax.
-
-Lemma mutualTiesSymmetric: forall program P P',
-  peers_tied program P P' -> peers_tied program P' P.
-Proof.
-  intros program P P' H_tied.
-  inversion H_tied.
-  unfold peers_tied; auto.
-Qed.
