TestSemanticsStatic.v
@@ -1,19 +1,6 @@
-Require Import ReTierStaticSemantics.
-Require Import ReTierSyntax.
-
-
-(* -------------------------------------------------------------------------
-  Tests for the ReTierStaticSemantics module
- * -------------------------------------------------------------------------*)
-
-
-
-
-
-(** In the following [plt_isWellTyped] and [has_type] are tested.
-  The tests are ordered such that every test case's proof only relies on tested
-  inference rules.
-**)
+Require Import Syntax.
+Require Import SemanticsStatic.
+Require Import Coq.Strings.String.
 
 
 Definition testPsi0: reactiveEnv := Datatypes.nil.
@@ -26,20 +13,124 @@ Definition testTies1 := Ties [
 Definition testPeerTyping1 := TypedInstances [
   4 : "pm", 3 : "po", 2 : "ps", 1 : "pn", 0 : "p0"].
 
+
+
+
+Example a1:
+  (Program NoTies NoTypedInstances) :: testPsi0; emptyPlaceEnv; emptyVarEnv; Peer "dummy"
+  |- lambda (Id "x") Unit (idApp (Id "x")) : Unit ~> Unit.
+Proof.
+apply T_Abs.
+apply T_Var.
+simpl.
+unfold idUpdate, Maps.p_update, Maps.t_update.
+destruct id_dec; try contradiction.
+left.
+reflexivity.
+Qed.
+
+Example a2:
+  (Program testTies1 testPeerTyping1) :: testPsi0; emptyPlaceEnv; emptyVarEnv; Peer "p0"
+  |- asLocalIn (Id "x") Unit unit (idApp (Id "x")) (Unit on (Peer "po")) : Option Unit.
+Proof.
+eapply T_Comp.
+- apply U_Unit.
+- apply U_Unit.
+- apply T_Unit.
+- apply T_Var.
+  simpl.
+  unfold idUpdate, Maps.p_update, Maps.t_update.
+  destruct id_dec; try contradiction.
+  left.
+  reflexivity.
+- cbv. split. + congruence. + congruence.
+- reflexivity.
+Qed.
+
+Example a3:
+  ~ (Program testTies1 testPeerTyping1) :: testPsi0; emptyPlaceEnv; emptyVarEnv; Peer "p0"
+    |- asLocalIn (Id "y") Unit unit (idApp (Id "x")) (Unit on (Peer "po")) : Option Unit.
+Proof.
+intro.
+inversion H.
+contradict H15.
+clear.
+intro.
+inversion H.
+contradict H6.
+clear.
+intro.
+destruct H.
+- unfold idUpdate, Maps.p_update, Maps.t_update in H.
+  case_eq (id_dec (Id "x") (Id "y")); intros H_eq.
+  + inversion H_eq.
+  + inversion H.
+- destruct H.
+  unfold emptyPlaceEnv, idEmpty, Maps.p_empty in H0.
+  inversion H0.
+Qed.
+
+
+Example a4:
+  (Program testTies1 testPeerTyping1) :: testPsi0; emptyPlaceEnv; emptyVarEnv; Peer "p0"
+  |- lambda (Id "x") Unit (asLocalIn (Id "x") Unit unit (idApp (Id "x")) (Unit on (Peer "po"))) : Unit ~> Option Unit.
+Proof.
+apply T_Abs.
+eapply T_Comp.
+- apply U_Unit.
+- apply U_Unit.
+- apply T_Unit.
+- apply T_Var.
+  simpl.
+  unfold idUpdate, Maps.p_update, Maps.t_update.
+  destruct id_dec; try contradiction.
+  left.
+  reflexivity.
+- cbv. split. + congruence. + congruence.
+- reflexivity.
+Qed.
+
+Example a5:
+  ~ (Program testTies1 testPeerTyping1) :: testPsi0; emptyPlaceEnv; emptyVarEnv; Peer "p0"
+    |- lambda (Id "x") Unit (asLocalIn (Id "y") Unit unit (idApp (Id "x")) (Unit on (Peer "po"))) : Unit ~> Option Unit.
+Proof.
+intro.
+inversion H.
+contradict H6.
+clear.
+intro.
+inversion H.
+contradict H15.
+clear.
+intro.
+inversion H.
+contradict H6.
+clear.
+intro.
+destruct H.
+- unfold
+    idUpdate, Maps.p_update, Maps.t_update,
+    emptyVarEnv, idEmpty, Maps.p_empty in H.
+  case_eq (id_dec (Id "x") (Id "y")); intros H_eq.
+  + inversion H_eq.
+  + inversion H.
+- destruct H.
+  unfold emptyPlaceEnv, idEmpty, Maps.p_empty in H0.
+  congruence.
+Qed.
+
+
 Example test_pltIsWellTyped_TEnd_1:
   (Program NoTies NoTypedInstances) :: testPsi0; emptyPlaceEnv |- pUnit.
 Proof. apply T_End. Qed.
-
 
 Example test_pltIsWellTyped_TEnd_2:
   (Program NoTies NoTypedInstances) :: testPsi1; testDelta1 |- pUnit.
 Proof. apply T_End. Qed.
 
-
 Example test_hasType_TUnit_1:
   (Program NoTies NoTypedInstances) :: testPsi0; emptyPlaceEnv; emptyVarEnv; Peer "dummy" |- unit : Unit.
 Proof. apply T_Unit. Qed.
-
 
 Example test_pltIsWellTyped_TPlace_1:
   (Program NoTies NoTypedInstances) :: testPsi1; testDelta1 |- placed (Id "x") (Unit on (Peer "px")) unit pUnit.
@@ -49,32 +140,25 @@ Proof.
   - apply T_Unit.
 Qed.
 
-
 Example test_hasType_TVar_normalVar_1:
   (Program NoTies NoTypedInstances) :: testPsi0; emptyPlaceEnv; testGamma1; Peer "p1" |- idApp (Id "x") : Tnat.
 Proof. apply T_Var. left. reflexivity. Qed.
-
 
 Example test_hasType_TVar_placedVar_2:
   (Program NoTies NoTypedInstances) :: testPsi0; testDelta1; emptyVarEnv; Peer "px" |- idApp (Id "x") : Unit.
 Proof. apply T_Var. right. split. - reflexivity. - reflexivity. Qed.
 
-
 Example test_hasType_TAbs_1: 
     (Program NoTies NoTypedInstances) :: testPsi0; emptyPlaceEnv; emptyVarEnv; Peer "dummy" |- lambda (Id "x") Tnat unit : Tnat ~> Unit.
 Proof. apply T_Abs. apply T_Unit. Qed.
-
 
 Example test_hasType_TAbs_2: 
     (Program NoTies NoTypedInstances) :: testPsi0; emptyPlaceEnv; emptyVarEnv; Peer "dummy" |- lambda (Id "x") Tnat (idApp (Id "x")) : Tnat ~> Tnat.
 Proof. apply T_Abs. apply T_Var. left. reflexivity. Qed.
 
-
-(** Tests variable shadowing **)
 Example test_hasType_TAbs_3:
   (Program NoTies NoTypedInstances) :: testPsi0; emptyPlaceEnv; testGamma1; Peer "_" |- lambda (Id "x") Unit (idApp (Id "x")) : Unit ~> Unit.
 Proof. apply T_Abs. apply T_Var. left. reflexivity. Qed.
-
 
 Example test_hasType_TApp_1:
   (Program NoTies NoTypedInstances) :: testPsi0; emptyPlaceEnv; emptyVarEnv; Peer "dummy" |- app (lambda (Id "x") Unit unit) unit : Unit.
@@ -84,7 +168,6 @@ Proof.
   - apply T_Unit.
 Qed.
 
-
 Example test_hasType_TApp_2: 
   (Program NoTies NoTypedInstances) :: testPsi0; emptyPlaceEnv; emptyVarEnv; Peer "dummy" |- app (lambda (Id "x") Unit (idApp (Id "x"))) unit : Unit.
 Proof.
@@ -93,11 +176,9 @@ Proof.
   - apply T_Unit.
 Qed.
 
-
 Example test_hasType_TNil_1: 
   (Program NoTies NoTypedInstances) :: testPsi0; emptyPlaceEnv; emptyVarEnv; Peer "dummy" |- nil Unit : List Unit.
 Proof. apply T_Nil. Qed.
-
 
 Example test_hasType_TCons_1: 
   (Program NoTies NoTypedInstances) :: testPsi0; emptyPlaceEnv; emptyVarEnv; Peer "dummy" |- cons unit (nil Unit) : List Unit.
@@ -107,31 +188,25 @@ Proof.
   - apply T_Nil.
 Qed.
 
-
 Example test_hasType_TSome_1: 
     (Program NoTies NoTypedInstances) :: testPsi0; emptyPlaceEnv; emptyVarEnv; Peer "dummy" |- some unit : Option Unit.
 Proof. apply T_Some. apply T_Unit. Qed.
-
 
 Example test_hasType_TNone_1: 
     (Program NoTies NoTypedInstances) :: testPsi0; emptyPlaceEnv; emptyVarEnv; Peer "dummy" |- none Unit : Option Unit.
 Proof. apply T_None. Qed.
 
-
 Example test_hasType_TPeer_1:
   (Program testTies1 testPeerTyping1) :: testPsi0; emptyPlaceEnv; emptyVarEnv; Peer "p0" |- peerApp (Instance 0) : Remote (Peer "p0").
 Proof. apply T_Peer. simpl. congruence. Qed.
 
-
 Example test_hasType_TAsLocal_single_1:
-  (* ensure test setup is correct ... *)
   testTies1 (Peer "p0", Peer "ps") = Single /\
-  (* actual test ... *)
   (Program testTies1 NoTypedInstances) :: testPsi0; emptyPlaceEnv; emptyVarEnv; Peer "p0"
     |- asLocal unit (Unit on (Peer "ps")) : Unit.
 Proof.
   split.
-  - reflexivity. (* ties set up correctly *)
+  - reflexivity.
   - apply T_AsLocal with (P0 := (Peer "p0")).
     + apply U_Unit.
     + apply T_Unit.
@@ -139,16 +214,13 @@ Proof.
     + reflexivity.
 Qed.
 
-
 Example test_hasType_TAsLocal_optional_1:
-  (* ensure test setup is correct ... *)
   testTies1 (Peer "p0", Peer "po") = Optional /\
-  (* actual test ... *)
   (Program testTies1 NoTypedInstances) :: testPsi0; emptyPlaceEnv; emptyVarEnv; Peer "p0"
     |- asLocal unit (Unit on (Peer "po")) : Option Unit.
 Proof.
   split.
-  - reflexivity. (* ties set up correctly *)
+  - reflexivity.
   - apply T_AsLocal with (P0 := (Peer "p0")).
     + apply U_Unit.
     + apply T_Unit.
@@ -156,16 +228,13 @@ Proof.
     + reflexivity.
 Qed.
 
-
 Example test_hasType_TAsLocal_multiple_1:
-  (* ensure test setup is correct ... *)
   testTies1 (Peer "p0", Peer "pm") = Multiple /\
-  (* actual test ... *)
   (Program testTies1 NoTypedInstances) :: testPsi0; emptyPlaceEnv; emptyVarEnv; Peer "p0"
     |- asLocal unit (Unit on (Peer "pm")) : List Unit.
 Proof.
   split.
-  - reflexivity.  (* current peer set correctly *)
+  - reflexivity.
   - apply T_AsLocal with (P0 := (Peer "p0")).
     + apply U_Unit.
     + apply T_Unit.
@@ -173,12 +242,9 @@ Proof.
     + reflexivity.
 Qed.
 
-
 Example test_hasType_TAsLocalFrom_single_1:
-  (* ensure test setup is correct ... *)
   typed_peer_instances_type testPeerTyping1 (PeerInstance 2) = Some (Peer "ps") /\
   testTies1 (Peer "p0", Peer "ps") = Single /\
-  (* actual test ... *)
   (Program testTies1 testPeerTyping1) :: testPsi0; emptyPlaceEnv; emptyVarEnv; Peer "p0"
     |- asLocalFrom unit (Unit on (Peer "ps")) (peerApp (Instance 2)) : Unit.
 Proof.
@@ -193,12 +259,9 @@ Proof.
       * apply T_Peer. simpl. congruence.
 Qed.
 
-
 Example test_hasType_TAsLocalFrom_optional_1:
-  (* ensure test setup is correct ... *)
   typed_peer_instances_type testPeerTyping1 (PeerInstance 3) = Some (Peer "po") /\
   testTies1 (Peer "p0", Peer "po") = Optional /\
-  (* actual test ... *)
   (Program testTies1 testPeerTyping1) :: testPsi0; emptyPlaceEnv; emptyVarEnv; Peer "p0"
     |- asLocalFrom unit (Unit on (Peer "po")) (peerApp (Instance 3)) : Unit.
 Proof.
@@ -213,12 +276,9 @@ Proof.
       * apply T_Peer. simpl. congruence.
 Qed.
 
-
 Example test_hasType_TAsLocalFrom_multiple_1:
-  (* ensure test setup is correct ... *)
   typed_peer_instances_type testPeerTyping1 (PeerInstance 4) = Some (Peer "pm") /\
   testTies1 (Peer "p0", Peer "pm") = Multiple /\
-  (* actual test ... *)
   (Program testTies1 testPeerTyping1) :: testPsi0; emptyPlaceEnv; emptyVarEnv; Peer "p0"
     |- asLocalFrom unit (Unit on (Peer "pm")) (peerApp (Instance 4)) : Unit.
 Proof.
@@ -233,11 +293,8 @@ Proof.
       * apply T_Peer. simpl. congruence.
 Qed.
 
-
 Example test_hasType_TComp_single_1:
-  (* ensure test setup is correct ... *)
   testTies1 (Peer "p0", Peer "ps") = Single /\
-  (* actual test ... *)
   (Program testTies1 NoTypedInstances) :: testPsi0; emptyPlaceEnv; emptyVarEnv; Peer "p0"
     |- asLocalIn (Id "x") Unit unit unit (Unit on (Peer "ps")) : Unit.
 Proof.
@@ -252,11 +309,8 @@ Proof.
     + reflexivity.
 Qed.
 
-
 Example test_hasType_TComp_optional_1:
-  (* ensure test setup is correct ... *)
   testTies1 (Peer "p0", Peer "po") = Optional /\
-  (* actual test ... *)
   (Program testTies1 NoTypedInstances) :: testPsi0; emptyPlaceEnv; emptyVarEnv; Peer "p0"
     |- asLocalIn (Id "x") Unit unit unit (Unit on (Peer "po")) : Option Unit.
 Proof.
@@ -271,11 +325,8 @@ Proof.
     + reflexivity.
 Qed.
 
-
 Example test_hasType_TComp_multiple_1:
-  (* ensure test setup is correct ... *)
   testTies1 (Peer "p0", Peer "pm") = Multiple /\
-  (* actual test ... *)
   (Program testTies1 NoTypedInstances) :: testPsi0; emptyPlaceEnv; emptyVarEnv; Peer "p0"
     |- asLocalIn (Id "x") Unit unit unit (Unit on (Peer "pm")) : List Unit.
 Proof.
@@ -290,11 +341,8 @@ Proof.
     + reflexivity.
 Qed.
 
-
 Example test_hasType_TComp_single_2:
-  (* ensure test setup is correct ... *)
   testTies1 (Peer "p0", Peer "ps") = Single /\
-  (* actual test ... *)
   (Program testTies1 NoTypedInstances) :: testPsi0; emptyPlaceEnv; emptyVarEnv; Peer "p0"
     |- asLocalIn (Id "x") Unit unit (idApp (Id "x")) (Unit on (Peer "ps")) : Unit.
 Proof.
@@ -309,12 +357,9 @@ Proof.
     + reflexivity.
 Qed.
 
-
 Example test_hasType_TCompFrom_single_1:
-  (* ensure test setup is correct ... *)
   typed_peer_instances_type testPeerTyping1 (PeerInstance 2) = Some (Peer "ps") /\
   testTies1 (Peer "p0", Peer "ps") = Single /\
-  (* actual test ... *)
   (Program testTies1 testPeerTyping1) :: testPsi0; emptyPlaceEnv; emptyVarEnv; Peer "p0"
     |- asLocalInFrom (Id "x") (*:*) Unit (*=*) unit (*in*) unit (*:*) (Unit on (Peer "ps"))
                      (*from*) (peerApp (Instance 2))
@@ -333,12 +378,9 @@ Proof.
       * apply T_Peer. simpl. congruence.
 Qed.
 
-
 Example test_hasType_TCompFrom_single_2:
-  (* ensure test setup is correct ... *)
   typed_peer_instances_type testPeerTyping1 (PeerInstance 2) = Some (Peer "ps") /\
   testTies1 (Peer "p0", Peer "ps") = Single /\
-  (* actual test ... *)
   (Program testTies1 testPeerTyping1) :: testPsi0; emptyPlaceEnv; emptyVarEnv; Peer "p0"
     |- asLocalInFrom (Id "x") (*:*) Unit (*=*) unit (*in*) (idApp (Id "x"))
                      (*:*) (Unit on (Peer "ps"))
@@ -358,11 +400,8 @@ Proof.
       * apply T_Peer. simpl. congruence.
 Qed.
 
-
 Example test_hasType_TReactive_1:
-  (* ensure test setup is correct ... *)
   reactive_type (Reactive 0) testPsi1 = Some (Signal Unit on Peer "_") /\
-  (* actual test ... *)
   (Program NoTies NoTypedInstances) :: testPsi1; emptyPlaceEnv; emptyVarEnv; Peer "_" |- reactApp (Reactive 0) : Signal Unit.
 Proof.
   split.
@@ -370,16 +409,13 @@ Proof.
   - apply T_Reactive with (T1 := Unit). + reflexivity. + left. reflexivity.
 Qed.
 
-
 Example test_hasType_TSignal_1:
   (Program NoTies NoTypedInstances) :: testPsi0; emptyPlaceEnv; emptyVarEnv; Peer "dummy" |- signal unit : Signal Unit.
 Proof. apply T_Signal. apply T_Unit. Qed.
 
-
 Example test_hasType_TReactiveVal_1:
   (Program NoTies NoTypedInstances) :: testPsi0; emptyPlaceEnv; emptyVarEnv; Peer "dummy" |- var unit : Var Unit.
 Proof. apply T_ReactiveVar. apply T_Unit. Qed.
-
 
 Example test_hasType_TNow_signal_1:
   (Program NoTies NoTypedInstances) :: testPsi0; emptyPlaceEnv; emptyVarEnv; Peer "dummy" |- now (signal unit) : Unit.
@@ -389,7 +425,6 @@ Proof.
   - left. reflexivity.
 Qed.
 
-
 Example test_hasType_TNow_var_1:
   (Program NoTies NoTypedInstances) :: testPsi0; emptyPlaceEnv; emptyVarEnv; Peer "dummy" |- now (var unit) : Unit.
 Proof.
@@ -398,7 +433,6 @@ Proof.
   - right. reflexivity.
 Qed.
 
-
 Example test_hasType_TSet_1:
   (Program NoTies NoTypedInstances) :: testPsi0; emptyPlaceEnv; emptyVarEnv; Peer "dummy" |- set (var unit) unit : Unit.
 Proof.
@@ -406,7 +440,6 @@ Proof.
   - apply T_ReactiveVar. apply T_Unit.
   - apply T_Unit.
 Qed.
-
 
 Example test_hasType_TSet_2:
   (Program NoTies NoTypedInstances) :: testPsi0; emptyPlaceEnv; emptyVarEnv; Peer "dummy"
@@ -421,4 +454,3 @@ Proof.
     + apply T_ReactiveVar. assumption.
     + assumption.
 Qed.
-
